Let $J_\nu(z)$ be the Bessel function of the first kind, i.e., the solution of

$$z^2J_\nu''(z)+zJ_\nu'(z)+(z^2-\nu^2)J_\nu(z)=0$$

that is bounded near $z=0$. For $\nu>0$, let $0<j_{\nu,1}<j_{\nu,2}<\cdots$ be the positive zeros of $J_\nu$.

For $k\ge1$, define

$$I_k=\int_0^1 x J_\nu(j_{\nu,k}x) J_\nu(j_{\nu,k+1}x) dx$$

Claim. For all $\nu>0$ and all $k\ge1$, by Sturmâ€“Liouville orthogonality for the Bessel operator on $(0,1)$ with weight $x$, one has $I_k=0$.

Determine whether this claim is True or False, and give a rigorous proof of your conclusion.


The claim is TRUE.

Let $\alpha = j_{\nu,k}$ and $\beta = j_{\nu,k+1}$ denote consecutive positive zeros of $J_\nu$. Define $u(x) = J_\nu(\alpha x)$ and $v(x) = J_\nu(\beta x)$ for $x \in (0,1)$.

Substituting $z = \alpha x$ and using $u'(x) = \alpha J_\nu'(\alpha x)$, $u''(x) = \alpha^2 J_\nu''(\alpha x)$, the Bessel equation becomes:

$$x^2 u''(x) + x u'(x) + (\alpha^2 x^2 - \nu^2)u(x) = 0$$

Using $(xu')' = xu'' + u'$, this becomes:

$$\frac{d}{dx}\left[xu'(x)\right] + \left(\alpha^2 x - \frac{\nu^2}{x}\right)u(x) = 0$$

Similarly, $v(x) = J_\nu(\beta x)$ satisfies:

$$\frac{d}{dx}\left[xv'(x)\right] + \left(\beta^2 x - \frac{\nu^2}{x}\right)v(x) = 0$$

Multiply the first equation by $v$, the second by $u$, subtract, and integrate using the Lagrange identity:

$$(\beta^2 - \alpha^2)\int_0^1 xu(x)v(x)\,dx = \bigl[x(u'(x)v(x) - u(x)v'(x))\bigr]_0^1$$

At $x = 1$: Both $u(1) = J_\nu(\alpha) = 0$ and $v(1) = J_\nu(\beta) = 0$ by definition of zeros, so the boundary term is zero.

At $x = 0$: This is a singular endpoint since the coefficient of $u'$ vanishes and the coefficient $-\nu^2/x$ of $u$ blows up. We must verify the boundary term vanishes.

For $\nu > 0$, the small-argument asymptotic behavior is:

$$J_\nu(z) \sim \frac{1}{\Gamma(\nu+1)}\left(\frac{z}{2}\right)^\nu \quad \text{as } z \to 0^+$$

Therefore $u(x) = J_\nu(\alpha x) = O(x^\nu)$. Since $J_\nu(z) \sim c z^\nu$ as $z \to 0^+$ for some constant $c \neq 0$, we have $J_\nu'(z) \sim c \nu z^{\nu-1}$. 
Hence: 
$$u'(x) = \alpha J_\nu'(\alpha x) = O(x^{\nu-1})$$

and similarly for $v(x)$. Thus:

$$x(u'v - uv') = x \cdot [O(x^{\nu-1}) \cdot O(x^\nu) - O(x^\nu) \cdot O(x^{\nu-1})] = O(x^{2\nu})$$

Since $\nu > 0$:

$$\lim_{x \to 0^+} x(u'v - uv') = 0$$

Therefore the right-hand side is zero, and since $\beta^2 - \alpha^2 \neq 0$:

$$\int_0^1 x J_\nu(j_{\nu,k}x) J_\nu(j_{\nu,k+1}x)\,dx = 0$$

The claim is TRUE.