Evaluate the integral
$$
I = \int_{0}^{\infty} e^{-x}\ x\ L_3(x)\ L_2^{(1)}(x)\ dx
$$
where $L_n(x)$ denotes the Laguerre polynomial with $\alpha = 0$ and $L_n^{(1)}(x)$ denotes the Laguerre polynomial with $\alpha = 1$.

1.	Identify the structure of the integral.
We want to evaluate
$$
I = \int_{0}^{\infty} e^{-x},x,L_3^{(0)}(x),L_2^{(1)}(x)\,dx.
$$
The factor $x e^{-x}$ is the orthogonality weight for Laguerre polynomials with $\alpha=1$.
2.	Apply the parameterâ€“shift identity.
For generalized Laguerre polynomials,
$$
L_n^{(\alpha-1)}(x) = L_n^{(\alpha)}(x) - L_{n-1}^{(\alpha)}(x).
$$
With $n=3,\ \alpha=1$:
$$
L_3^{(0)}(x) = L_3^{(1)}(x) - L_2^{(1)}(x).
$$
3.	Substitute into the integral.
$$
I = \int_{0}^{\infty} x e^{-x}[L_3^{(1)}(x)-L_2^{(1)}(x)]L_2^{(1)}(x)\,dx.
$$
This splits as
$$
I = \int_{0}^{\infty} x e^{-x}L_3^{(1)}(x)L_2^{(1)}(x)\,dx \,-\,\int_{0}^{\infty} x e^{-x}[L_2^{(1)}(x)]^2\,dx.
$$
4.	Apply orthogonality.
For Laguerre polynomials with $\alpha=1$:
$$
\int_{0}^{\infty} x e^{-x} L_m^{(1)}(x) L_n^{(1)}(x),dx = \frac{\Gamma(n+2)}{n!}\,\delta_{mn}.
$$
Therefore, the cross term with $m=2$ and $n=3$ vanishes.

5.	Evaluate the square norm.
$$
\int_{0}^{\infty} x e^{-x}[L_2^{(1)}(x)]^2 dx = \frac{\Gamma(4)}{2!} = 3.
$$
6.	Final result.
$$
I = 0 - 3 = -3.
$$