
Let $Y_{\ell m}(\theta\,\phi)$ denote the standard spherical harmonics on the unit sphere $\mathbb{S}^2$ with normalization
$$Y_{\ell m}(\theta\,\phi) = \sqrt{\frac{2\ell+1}{4\pi}\frac{(\ell-m)!}{(\ell+m)!}} P_{\ell}^m(\cos\theta) e^{im\phi}$$
where $P_{\ell}^m$ are the associated Legendre functions and $(\theta\,\phi) \in [0\,\pi] \times [0\,2\pi)$.

The angular momentum raising operator is defined by
$$L_+ Y_{\ell m} = \sqrt{(\ell-m)(\ell+m+1)} \, Y_{\ell\,m+1}$$

For fixed degree $\ell \geq 1$ and magnetic quantum number $m$ with $-\ell \leq m < \ell$, consider the quantity
$$R_{\ell m}(\theta) = \frac{1}{\sin\theta} \frac{\partial Y_{\ell m}(\theta\,0)}{\partial\theta}$$

Claim

For all integers $\ell \geq 1$ and all $m$ with $-\ell \leq m < \ell$, the limit
$$\lim_{\theta \to 0} \frac{R_{\ell m}(\theta)}{Y_{\ell\,m+1}(\theta\,0)} = \sqrt{(\ell-m)(\ell+m+1)}$$
exists and equals the raising operator coefficient.

Determine with rigorous proof whether the claim is True or False.


Claim: FALSE

The angular momentum raising operator in spherical coordinates is:
$$L_+ = e^{i\phi}\left(\frac{\partial}{\partial\theta} + i\cot\theta\frac{\partial}{\partial\phi}\right)$$

For spherical harmonics $Y_{\ell m}(\theta\,\phi) = \Theta_{\ell m}(\theta) e^{im\phi}$, the derivative with respect to $\phi$ gives $\frac{\partial Y_{\ell m}}{\partial\phi} = im Y_{\ell m}$. Applying the raising operator at $\phi=0$:

$$L_+ Y_{\ell m}\big|_{\phi=0} = e^{i \cdot 0}\left(\frac{\partial Y_{\ell m}(\theta\,0)}{\partial\theta} + i\cot\theta \cdot im Y_{\ell m}(\theta\,0)\right) = \frac{\partial Y_{\ell m}(\theta\,0)}{\partial\theta} - m\cot\theta Y_{\ell m}(\theta\,0)$$

Using the ladder relation $L_+ Y_{\ell m} = \sqrt{(\ell-m)(\ell+m+1)} \, Y_{\ell\,m+1}$:

$$\frac{\partial Y_{\ell m}(\theta\,0)}{\partial\theta} = \sqrt{(\ell-m)(\ell+m+1)} \, Y_{\ell\,m+1}(\theta\,0) + m\cot\theta \, Y_{\ell m}(\theta\,0)$$

Expressing $R_{\ell m}(\theta) = \frac{1}{\sin\theta}\frac{\partial Y_{\ell m}(\theta\,0)}{\partial\theta}$:

$$R_{\ell m}(\theta) = \frac{\sqrt{(\ell-m)(\ell+m+1)} \, Y_{\ell\,m+1}(\theta\,0)}{\sin\theta} + \frac{m\cos\theta}{\sin^2\theta} Y_{\ell m}(\theta\,0)$$

Consider the specific case $\ell = 1$, $m = 0$. Here $Y_{10}(\theta\,0) = \sqrt{\frac{3}{4\pi}} \cos\theta$ and $Y_{11}(\theta\,0) = -\sqrt{\frac{3}{8\pi}} \sin\theta$. The derivative is $\frac{\partial Y_{10}}{\partial\theta} = -\sqrt{\frac{3}{4\pi}} \sin\theta$, so:

$$R_{10}(\theta) = \frac{1}{\sin\theta}\left(-\sqrt{\frac{3}{4\pi}} \sin\theta\right) = -\sqrt{\frac{3}{4\pi}}$$

This is constant. The ratio becomes:

$$\frac{R_{10}(\theta)}{Y_{11}(\theta\,0)} = \frac{-\sqrt{\frac{3}{4\pi}}}{-\sqrt{\frac{3}{8\pi}} \sin\theta} = \frac{\sqrt{2}}{\sin\theta}$$

As $\theta \to 0$, this gives $\lim_{\theta \to 0} \frac{\sqrt{2}}{\sin\theta} = +\infty$, not the claimed value $\sqrt{2}$.

The claim is false. The extra factor $1/\sin\theta$ in the definition of $R_{\ell m}$ introduces a singularity at $\theta=0$, so the ratio need not have a finite limit even though the ladder identity holds for $L_+$.