Let $Y_{\ell m}(\theta,\phi)$ denote the standard spherical harmonics on $\mathbb{S}^2$, normalized in $L^2(\mathbb{S}^2)$, with integers $\ell \geq 0$ and $|m| \leq \ell$. The addition theorem for spherical harmonics states

$$P_\ell(\cos\omega) = \frac{4\pi}{2\ell+1} \sum_{m=-\ell}^{\ell} Y_{\ell m}(\theta_1,\phi_1) \overline{Y_{\ell m}(\theta_2,\phi_2)}$$

where $P_\ell$ are the Legendre polynomials and $\omega$ is the angle between the points $(\theta_1,\phi_1)$ and $(\theta_2,\phi_2)$ on the sphere, given by

$$\cos\omega = \cos\theta_1\cos\theta_2 + \sin\theta_1\sin\theta_2\cos(\phi_1-\phi_2)$$

For fixed $\ell \geq 1$, define the modified sum

$$S_\ell(\theta_1,\phi_1,\theta_2,\phi_2) = \sum_{m=-\ell}^{\ell} (-1)^m Y_{\ell m}(\theta_1,\phi_1) \overline{Y_{\ell m}(\theta_2,\phi_2)}$$

Claim: For all points $(\theta_1,\phi_1)$ and $(\theta_2,\phi_2)$ on the sphere, the modified sum satisfies

$$S_\ell(\theta_1,\phi_1,\theta_2,\phi_2) = \frac{2\ell+1}{4\pi} P_\ell(-\cos\omega)$$

Determine whether this claim is True or False, and give a rigorous proof of your conclusion.

The claim is False.

We establish this by considering the special case where both points coincide on the north pole: $(\theta_1,\phi_1) = (\theta_2,\phi_2) = (0,0)$. In this case, $\omega = 0$, so $\cos\omega = 1$ and $-\cos\omega = -1$.

At the north pole $\theta = 0$, the spherical harmonics simplify significantly. The normalized spherical harmonics are

$$Y_{\ell m}(\theta,\phi) = \sqrt{\frac{2\ell+1}{4\pi}\frac{(\ell-m)!}{(\ell+m)!}} P_{\ell}^{m}(\cos\theta) e^{im\phi}$$

where $P_{\ell}^m$ are the associated Legendre functions. At $\theta = 0$, we have $\cos\theta = 1$, and by standard properties of associated Legendre functions,

$$P_{\ell}^m(1) = \begin{cases} 1 & \text{if } m = 0 \\ 0 & \text{if } m \neq 0 \end{cases}$$

Therefore, at the north pole,

$$Y_{\ell m}(0,0) = \begin{cases} \sqrt{\frac{2\ell+1}{4\pi}} & \text{if } m = 0 \\ 0 & \text{if } m \neq 0 \end{cases}$$

The modified sum at coincident north pole points becomes

$$S_\ell(0,0,0,0) = \sum_{m=-\ell}^{\ell} (-1)^m |Y_{\ell m}(0,0)|^2 = (-1)^0 \left(\sqrt{\frac{2\ell+1}{4\pi}}\right)^2 = \frac{2\ell+1}{4\pi}$$

since only the $m = 0$ term survives and $(-1)^0 = 1$.

According to the claim, this should equal

$$\frac{2\ell+1}{4\pi} P_\ell(-1)$$

For the Legendre polynomial $P_\ell(x)$, we have the well-known value

$$P_\ell(-1) = (-1)^\ell$$

Therefore, the claimed value is

$$\frac{2\ell+1}{4\pi} P_\ell(-1) = \frac{2\ell+1}{4\pi} (-1)^\ell$$

Comparing, we need

$$\frac{2\ell+1}{4\pi} = \frac{2\ell+1}{4\pi} (-1)^\ell$$

which requires $(-1)^\ell = 1$, i.e., $\ell$ must be even. For odd $\ell$, we have $(-1)^\ell = -1$, giving

$$S_\ell(0,0,0,0) = \frac{2\ell+1}{4\pi} \neq \frac{2\ell+1}{4\pi}(-1) = -\frac{2\ell+1}{4\pi}$$

Taking $\ell = 1$ as a concrete counterexample, $S_1(0,0,0,0) = \frac{3}{4\pi}$ but the claimed value is $\frac{3}{4\pi} \cdot (-1) = -\frac{3}{4\pi}$, establishing that the claim is false.