
Let $D_{mm'}^{\ell}(\alpha,\beta,\gamma)$ denote the Wigner D-functions (generalized spherical harmonics) which describe how spherical harmonics transform under rotations specified by Euler angles $(\alpha,\beta,\gamma)$. These functions can be factored as

$$D_{mm'}^{\ell}(\alpha,\beta,\gamma) = e^{i(m\alpha + m'\gamma)} d_{mm'}^{\ell}(\beta)$$

where $d_{mm'}^{\ell}(\beta)$ are real-valued functions. The Wigner D-functions satisfy the orthogonality relation

$$\frac{1}{8\pi^2} \int_0^{2\pi} \int_0^{\pi} \int_0^{2\pi} D_{m_1 m_1'}^{\ell}(\alpha,\beta,\gamma) \overline{D_{m_2 m_2'}^{\ell}(\alpha,\beta,\gamma)} \sin\beta \, d\alpha \, d\beta \, d\gamma = \frac{1}{2\ell+1} \delta_{m_1 m_2} \delta_{m_1' m_2'}$$

and the completeness relation (unitarity of rotation matrices)

$$\sum_{m=-\ell}^{\ell} d_{mm_1}^{\ell}(\beta) d_{mm_2}^{\ell}(\beta) = \delta_{m_1 m_2}$$

For fixed $\ell \geq 1$, define the weighted average

$$\bar{S}_{\ell} = \frac{1}{2} \int_0^{\pi} \left[\sum_{m=-\ell}^{\ell} d_{m,0}^{\ell}(\beta) d_{0,m}^{\ell}(\beta)\right] \sin\beta \, d\beta$$

Claim: The weighted average $\bar{S}_{\ell}$ equals

$$\bar{S}_{\ell} = \frac{1}{2\ell+1}$$

Determine whether this claim is True or False, and give a rigorous proof of your conclusion.


The claim is False.

Let $d^{\ell}(\beta)$ be the real $(2\ell+1) \times (2\ell+1)$ matrix with entries $d_{mm'}^{\ell}(\beta)$. The composition law for rotations about the $y$-axis gives

$$d^{\ell}(\beta_1) d^{\ell}(\beta_2) = d^{\ell}(\beta_1 + \beta_2)$$

By commutativity of multiplication of real numbers, we have

$$\sum_{m=-\ell}^{\ell} d_{m,0}^{\ell}(\beta) d_{0,m}^{\ell}(\beta) = \sum_{m=-\ell}^{\ell} d_{0,m}^{\ell}(\beta) d_{m,0}^{\ell}(\beta) = \left(d^{\ell}(\beta)^2\right)_{00} = d_{00}^{\ell}(2\beta)$$


where the last equality follows from the composition law. For the $y$-axis rotation convention, it is standard that $d_{00}^{\ell}(\beta) = P_{\ell}(\cos\beta)$, where $P_{\ell}$ are the Legendre polynomials. Therefore the integrand equals $P_{\ell}(\cos 2\beta)$, and

$$\bar{S}_{\ell} = \frac{1}{2} \int_0^{\pi} P_{\ell}(\cos 2\beta) \sin\beta \, d\beta$$

We compute this for $\ell = 1$, where $P_1(t) = t$. Then

$$\bar{S}_1 = \frac{1}{2} \int_0^{\pi} \cos 2\beta \sin\beta \, d\beta$$

Substituting $u = \cos\beta$ gives $\cos 2\beta = 2u^2 - 1$ and $\sin\beta \, d\beta = -du$. The limits transform as $\beta: 0 \to \pi$ corresponds to $u: 1 \to -1$, so

$$\bar{S}_1 = \frac{1}{2} \int_{1}^{-1} (2u^2 - 1)(-du) = \frac{1}{2} \int_{-1}^{1} (2u^2 - 1) du$$

Evaluating,

$$\bar{S}_1 = \frac{1}{2} \left[2 \cdot \frac{2}{3} - 2\right] = \frac{1}{2} \left[\frac{4}{3} - 2\right] = \frac{1}{2} \cdot \left(-\frac{2}{3}\right) = -\frac{1}{3}$$

However, the claimed value is $\frac{1}{2\ell+1} = \frac{1}{3}$ for $\ell = 1$. Since $\bar{S}_1 = -\frac{1}{3} \neq \frac{1}{3}$, the claim is false.