The Legendre polynomials $P_n(x)$ have the generating function:

$$\frac{1}{\sqrt{1 - 2tx + t^2}} = \sum_{n=0}^{\infty} P_n(x) t^n$$

for $|t| < 1$ and $x \in [-1,1]$.

For fixed $x_0 \in (0,1)$ and $n \geq 1$, consider the weighted sum:

$$S_N(x_0) = \sum_{n=1}^{N} \frac{P_n(x_0)}{n!}$$

Claim: For all $x_0 \in (0,1)$, the series $\sum_{n=1}^{\infty} \frac{P_n(x_0)}{n!}$ converges, and the sum satisfies:

$$\sum_{n=1}^{\infty} \frac{P_n(x_0)}{n!} = e^{x_0} - 1$$

Determine with rigorous proof whether the claim is True or False.

The claim is False

Since Legendre polynomials satisfy $|P_n(x)| \leq 1$ for all $n \geq 0$ and all $x \in [-1,1]$ (the maximum is 1, attained at $x = \pm 1$), the series converges absolutely by comparison with $\sum_{n=1}^{\infty} \frac{1}{n!} = e - 1$.

To disprove the claim, consider $x_0 = 1/2$. Using $P_2(x) = \frac{1}{2}(3x^2 - 1)$:

$$P_2(1/2) = \frac{1}{2}\left(\frac{3}{4} - 1\right) = -\frac{1}{8}$$

The $n=2$ term of the series is:

$$\frac{P_2(1/2)}{2!} = \frac{-1/8}{2} = -\frac{1}{16}$$

But the $n=2$ term of $e^{x_0} - 1 = e^{1/2} - 1$ is:

$$\frac{(1/2)^2}{2!} = \frac{1}{8}$$

Since $-\frac{1}{16} \neq \frac{1}{8}$, the series cannot equal $e^{x_0} - 1$ at $x_0 = 1/2$.

Therefore the claim is false.