Consider the monic Laguerre polynomials $p_n(x)$ on $[0, \infty)$ with weight $\rho(x) = e^{-x}$, where $p_n(x) = (-1)^n n! L_n(x)$ and $L_n$ is the standard Laguerre polynomial ($\alpha = 0$). For each $n \ge 0$ and $z \in \mathbb{C} \setminus [0, \infty)$ define the second order Cauchy transform

$$\tilde q_n(z) = \int_0^\infty \frac{p_n(x)e^{-x}}{(z-x)^2} dx$$

Fix $n \ge 1$ and set

$$\tilde{\bar q}_n(z) = \tilde q_n(z)p_{n-1}(z) - \tilde q_{n-1}(z)p_n(z)$$

Claim: $\tilde{\bar q}_n(z)$ is independent of $z$ on $\mathbb{C} \setminus [0, \infty)$. Determine, with rigorous proof, whether the claim is True or False.


----------

The claim is False.

Step 1. For each $n \ge 0$ and $z \in \mathbb{C} \setminus [0, \infty)$ define $q_n(z) = \int_0^\infty \frac{p_n(x) e^{-x}}{z - x}\,dx$. Let $K \subset \mathbb{C} \setminus [0, \infty)$ be compact and let $d = \text{dist}(K, [0, \infty)) > 0$. For $z \in K$ and $x \ge 0$ we have $|z - x| \ge d$, hence $|(z - x)^{-2}| \le d^{-2}$. Since $p_n$ is a polynomial of degree $n$, there exists $C > 0$ such that $|p_n(x)| \le C(1 + x^n)$ for $x \ge 0$. Therefore for $z \in K$ and $x \ge 0$,

$$\left|\partial_z \frac{p_n(x) e^{-x}}{z - x}\right| = \left|\frac{-p_n(x) e^{-x}}{(z - x)^2}\right| \le \frac{C(1+x^n)e^{-x}}{d^2}$$

and the right-hand side is integrable on $[0, \infty)$. By dominated convergence, differentiation under the integral sign is valid and $r_n(z) = q_n'(z) = -\int_0^\infty \frac{p_n(x) e^{-x}}{(z - x)^2}\,dx$.

Step 2. Take $n = 1$. Then $p_0(x) = 1$ and $p_1(x) = x - 1$. Define $q_0(z) = \int_0^\infty \frac{e^{-x}}{z - x}\,dx$. Using $x - 1 = (z - 1) - (z - x)$, we have:

$$\begin{aligned} q_1(z) &= \int_0^\infty \frac{(x - 1) e^{-x}}{z - x}\,dx \\ &= \int_0^\infty \frac{(z - 1) - (z - x)}{z - x} e^{-x}\,dx \\ &= (z - 1) \int_0^\infty \frac{e^{-x}}{z - x}\,dx - \int_0^\infty \frac{(z - x) e^{-x}}{z - x}\,dx \\ &= (z - 1) q_0(z) - \int_0^\infty e^{-x}\,dx \\ &= (z - 1) q_0(z) - 1 \end{aligned}$$

Step 3. Differentiate $q_1(z) = (z - 1) q_0(z) - 1$ to get $r_1(z) = q_1'(z) = q_0(z) + (z - 1) r_0(z)$. Then, using $p_0(z) = 1$ and $p_1(z) = z - 1$:

$$\begin{aligned} \bar r_1(z) &= r_1(z) p_0(z) - r_0(z) p_1(z) \\ &= [q_0(z) + (z - 1) r_0(z)](1) - r_0(z)(z - 1) \\ &= q_0(z) + (z - 1) r_0(z) - (z - 1) r_0(z) \\ &= q_0(z) \end{aligned}$$

Step 4. Show $q_0$ is not constant on $\mathbb{C} \setminus [0, \infty)$. Pick $z_1 = -1$ and $z_2 = -2$, both in $\mathbb{C} \setminus [0, \infty)$. For every $x \ge 0$, we have:

$$\frac{1}{-1 - x} < \frac{1}{-2 - x} < 0$$

Multiplying by $e^{-x} > 0$ and integrating over $[0, \infty)$ gives:

$$\begin{aligned} q_0(-1) &= \int_0^\infty \frac{e^{-x}}{-1 - x}\,dx \\ &< \int_0^\infty \frac{e^{-x}}{-2 - x}\,dx \\ &= q_0(-2) \end{aligned}$$

Hence $q_0$ is not constant, so $\bar r_1(z) = q_0(z)$ is not constant. Therefore $\bar r_n(z)$ is not independent of $z$ in general, and the claim is false.