Let $\nu>0$ and let $J_\nu$ be the Bessel function of the first kind. For $z_1>0$ define $z_2=z_1+2\pi$ and, whenever $J_\nu(z_1)J_\nu(z_2)\neq0$, define

$$\Phi_\nu(z_1,z_2)=\frac{J_\nu(z_1)J_\nu'(z_2)-J_\nu'(z_1)J_\nu(z_2)}{J_\nu(z_1)J_\nu(z_2)}.$$

Claim: For every $\nu\ge1$ there exists a constant $C_\nu>0$ such that for all $z_1\ge2\nu$ with $J_\nu(z_1)J_\nu(z_1+2\pi)\neq0$ one has

$$\bigl|\Phi_\nu(z_1,z_1+2\pi)\bigr|\le\frac{C_\nu}{\sqrt{z_1}}.$$

The claim is false.

Step 1. Fix $\nu \ge 1$. Let $j_{\nu,k}$ denote the $k$-th positive zero of $J_\nu$. It is a standard result that $J_\nu$ has infinitely many positive zeros and each is simple, so $J_\nu(j_{\nu,k}) = 0$ and $J_\nu'(j_{\nu,k}) \neq 0$.

Step 2. For sufficiently large $k$, $J_\nu(j_{\nu,k} + 2\pi) \neq 0$. This is established by proving the point lies strictly between consecutive zeros. The asymptotic expansion for the zeros is

$$j_{\nu,k} = \Bigl(k + \frac{\nu}{2} - \frac{1}{4}\Bigr)\pi - \frac{4\nu^2 - 1}{8(k + \frac{\nu}{2} - \frac{1}{4})\pi} + O(k^{-3}).$$

The difference $j_{\nu,k+2} - j_{\nu,k} = 2\pi + \mathcal{O}(k^{-2})$. Define $\delta_k = (j_{\nu,k} + 2\pi) - j_{\nu,k+2}$, such that $\delta_k = O(k^{-2})$. Since $j_{\nu,n+1} - j_{\nu,n} \to \pi$, there exist $c > 0$ and $n_0$ such that for all $n \ge n_0$, $j_{\nu,n+1} - j_{\nu,n} \ge c$. For $k$ large enough, this lower bound applies to the adjacent gaps $(j_{\nu,k+1}, j_{\nu,k+2})$ and $(j_{\nu,k+2}, j_{\nu,k+3})$. Choose $k$ large enough so that $|\delta_k| < c/2$.

If $\delta_k > 0$, then $j_{\nu,k} + 2\pi \in (j_{\nu,k+2}, j_{\nu,k+3})$.

If $\delta_k < 0$, then $j_{\nu,k} + 2\pi \in (j_{\nu,k+1}, j_{\nu,k+2})$.

In either case, $j_{\nu,k} + 2\pi$ lies strictly between consecutive zeros, ensuring $J_\nu(j_{\nu,k} + 2\pi) \neq 0$.

Step 3. Fix $x = j_{\nu,k}$ such that $x \ge 2\nu$ and $J_\nu(y) \neq 0$ where $y = x+2\pi$. Since $x$ is a simple zero, there exists $\eta_1 > 0$ such that $J_\nu(x+\varepsilon) \neq 0$ for all $0 < |\varepsilon| < \eta_1$. By continuity at $y$, there exists $\eta_2 > 0$ such that for $|\varepsilon| < \eta_2$

$$|J_\nu(y+\varepsilon) - J_\nu(y)| \le \frac{|J_\nu(y)|}{2}.$$

By the reverse triangle inequality, $|J_\nu(y+\varepsilon)| \ge |J_\nu(y)|/2 > 0$. Therefore, for $0 < |\varepsilon| < \min(\eta_1, \eta_2)$, we have $J_\nu(z_1) \neq 0$ and $J_\nu(z_2) = J_\nu(z_1+2\pi) \neq 0$, and moreover $|J_\nu(z_2)| \ge |J_\nu(y)|/2$, so $\Phi_\nu(z_1,z_2)$ is well defined and division by $J_\nu(z_1)J_\nu(z_2)$ is legitimate.

Step 4. Let $z_1 = x+\varepsilon$ and $z_2 = y+\varepsilon$. The expansions around $x$ and $y$ are

$J_\nu(z_1) = J_\nu'(x)\varepsilon + R_1$, where $R_1 = O(\varepsilon^2)$

$J_\nu'(z_1) = J_\nu'(x) + R_2$, where $R_2 = O(\varepsilon)$

$J_\nu(z_2) = J_\nu(y) + R_3$, where $R_3 = O(\varepsilon)$

$J_\nu'(z_2) = J_\nu'(y) + R_4$, where $R_4 = O(\varepsilon)$.

For the numerator $N$

$$N = (J_\nu'(x)\varepsilon + R_1)(J_\nu'(y) + R_4) - (J_\nu'(x) + R_2)(J_\nu(y) + R_3).$$

The first product $(J_\nu'(x)\varepsilon + R_1)(J_\nu'(y) + R_4) = J_\nu'(x)J_\nu'(y)\varepsilon + O(\varepsilon^2) = O(\varepsilon)$.

The second product $(J_\nu'(x) + R_2)(J_\nu(y) + R_3) = J_\nu'(x)J_\nu(y) + O(\varepsilon)$.

Hence, $N = -J_\nu'(x)J_\nu(y) + O(\varepsilon)$.

For the denominator $D$

$$D = (J_\nu'(x)\varepsilon + R_1)(J_\nu(y) + R_3) = J_\nu'(x)J_\nu(y)\varepsilon + O(\varepsilon^2).$$

Step 5. Since $J_\nu'(x) \neq 0$ and $J_\nu(y) \neq 0$

$$\Phi_\nu(z_1, z_2) = \frac{-J_\nu'(x)J_\nu(y) + O(\varepsilon)}{J_\nu'(x)J_\nu(y)\varepsilon + O(\varepsilon^2)} = -\frac{1}{\varepsilon} + O(1).$$

As $\varepsilon \to 0$, $|\Phi_\nu| \to \infty$. Thus, for any $C_\nu$, there exists $\varepsilon$ small enough such that $|\Phi_\nu(x+\varepsilon, x+2\pi+\varepsilon)| > \frac{C_\nu}{\sqrt{x+\varepsilon}}$. Therefore, the claim is false.