Let $L_n^{(\alpha)}(x)$ denote the standard (non-monic) generalized Laguerre polynomials with $\alpha > -1$, orthogonal on $[0, \infty)$ with respect to the weight $x^\alpha e^{-x}$.

For $z \in \mathbb{C} \setminus [0, \infty)$, define the function of the second kind by

$$Q_n^{(\alpha)}(z) = \int_0^\infty \frac{L_n^{(\alpha)}(s) s^\alpha e^{-s}}{z - s} ds.$$

For $n \ge 1$, define

$$\Phi_n^{(\alpha)}(z) = L_n^{(\alpha)}(z) Q_{n-1}^{(\alpha)}(z) - L_{n-1}^{(\alpha)}(z) Q_n^{(\alpha)}(z).$$

Claim.

For every $n \ge 1$, the function $\Phi_n^{(\alpha)}(z)$ is independent of $z$ on $\mathbb{C} \setminus [0, \infty)$ and satisfies

$$\Phi_n^{(\alpha)}(z) = -\frac{\Gamma(n + \alpha)}{n!}.$$

Determine, with rigorous proof, whether the claim is True or False.

Conclusion: True

Step 1.

Define the monic Laguerre polynomials on $[0, \infty)$ by

$$\pi_n(x) = (-1)^n n! L_n^{(\alpha)}(x)$$

Since $L_n^{(\alpha)}(x)$ has leading term $(-1)^n x^n/n!$, the polynomial $\pi_n$ is monic. They satisfy the orthogonality relation

$$\int_0^\infty \pi_n(s) \pi_m(s) s^\alpha e^{-s} ds = h_n \delta_{nm}$$

The monic squared norm is given by

$$h_n = n! \Gamma(n + \alpha + 1)$$

In particular, the monic squared norm for index $n-1$ is

$$h_{n-1} = (n - 1)! \Gamma(n + \alpha)$$

For $z \in \mathbb{C} \setminus [0, \infty)$ define the second-kind transform for the monic family by

$$q_n(z) = \int_0^\infty \frac{\pi_n(s) s^\alpha e^{-s}}{z - s} ds$$

From the definition of $\pi_n$, the transform relation is immediate:

$$q_n(z) = (-1)^n n! Q_n^{(\alpha)}(z)$$

Step 2.

The Christoffel-Darboux formula for the monic Laguerre polynomials is

$$\sum_{k=0}^{n-1} \frac{\pi_k(s) \pi_k(z)}{h_k} = \frac{\pi_n(s) \pi_{n-1}(z) - \pi_{n-1}(s) \pi_n(z)}{h_{n-1} (s - z)}$$

Multiply both sides by $s^\alpha e^{-s}$ and integrate over $(0, \infty)$. Since the sum is finite, the interchange of summation and integration is valid. On the left:

$$\sum_{k=0}^{n-1} \frac{\pi_k(z)}{h_k} \int_0^\infty \pi_k(s) s^\alpha e^{-s} ds$$

By orthogonality, the integrals vanish for all $k \ge 1$. For $k = 0$, $\pi_0 = 1$ and $h_0 = \Gamma(\alpha + 1)$, so:

$$\frac{1}{h_0} \int_0^\infty s^\alpha e^{-s} ds = \frac{1}{\Gamma(\alpha + 1)} \Gamma(\alpha + 1) = 1$$

On the right-hand side, using the identity $1 / (s - z) = -1 / (z - s)$, we obtain:

$$\int_0^\infty \frac{\pi_m(s) s^\alpha e^{-s}}{s - z} ds = -q_m(z)$$

Applying this to the right-hand side of the Christoffel-Darboux integral:

$$1 = \frac{\pi_n(z) q_{n-1}(z) - \pi_{n-1}(z) q_n(z)}{h_{n-1}}$$

Thus:

$$\pi_n(z) q_{n-1}(z) - \pi_{n-1}(z) q_n(z) = h_{n-1}$$

Step 3.

Using the relations from Step 1, we convert the monic identity back to the standard Laguerre form:

$$\pi_n(z) q_{n-1}(z) - \pi_{n-1}(z) q_n(z) = (-1)^n n! L_n^{(\alpha)}(z) \cdot (-1)^{n-1} (n - 1)! Q_{n-1}^{(\alpha)}(z) - (-1)^{n-1} (n - 1)! L_{n-1}^{(\alpha)}(z) \cdot (-1)^n n! Q_n^{(\alpha)}(z)$$

Both terms carry the sign $(-1)^n \cdot (-1)^{n-1} = -1$. Factoring the constants yields:

$$\pi_n q_{n-1} - \pi_{n-1} q_n = -n! (n - 1)! \left( L_n^{(\alpha)}(z) Q_{n-1}^{(\alpha)}(z) - L_{n-1}^{(\alpha)}(z) Q_n^{(\alpha)}(z) \right)$$

$$\pi_n q_{n-1} - \pi_{n-1} q_n = -n! (n - 1)! \Phi_n^{(\alpha)}(z)$$

Equating this with the result of Step 2 gives:

$$-n! (n - 1)! \Phi_n^{(\alpha)}(z) = h_{n-1}$$

Step 4.

Substituting $h_{n-1} = (n - 1)! \Gamma(n + \alpha)$ yields:

$$\Phi_n^{(\alpha)}(z) = -\frac{(n - 1)! \Gamma(n + \alpha)}{n! (n - 1)!}$$

$$\Phi_n^{(\alpha)}(z) = -\frac{\Gamma(n + \alpha)}{n!}$$

This value is independent of $z$ on $\mathbb{C} \setminus [0, \infty)$ and coincides with the claimed constant.

Final Answer: True.