Let $H_n(x)$ be the physicist's Hermite polynomials. For $z \in \mathbb{C} \setminus \mathbb{R}$, define the function of the second kind $Q_n(z)$ by the integral representation:

$$Q_n(z) = e^{z^2} \int_{-\infty}^\infty \frac{H_n(s) e^{-s^2}}{s-z} ds$$

Consider the sequence of functions $\{\Phi_n(z)\}_{n \ge 1}$ defined by the combination:

$$\Phi_n(z) = Q_n(z)H_{n-1}(z) - Q_{n-1}(z)H_n(z)$$

Claim: For every $n \ge 1$, the function $\Phi_n(z)$ satisfies the asymptotic limit

$$\lim_{|z| \to \infty} e^{-z^2} \Phi_n(z) = 2^n (n-1)! \sqrt{\pi}$$

Determine, with rigorous proof, whether the claim is True or False.

----------
Conclusion: True

Step 1. Define the monic Hermite polynomials by

$$\pi_n(x) = 2^{-n}H_n(x)$$

They satisfy the orthogonality relation

$$\int_{-\infty}^{\infty} \pi_n(s) \pi_m(s) e^{-s^2} ds = h_n \delta_{nm}$$

where

$$h_n = 2^{-n} n! \sqrt{\pi}$$

For $z \in \mathbb{C} \setminus \mathbb{R}$, define the function of the second kind

$$q_n(z) = \int_{-\infty}^{\infty} \frac{\pi_n(s) e^{-s^2}}{z - s} ds$$

The given function $Q_n$ satisfies

$$Q_n(z) = -e^{z^2} 2^n q_n(z)$$

since $1/(s - z) = -1/(z - s)$.

Step 2. For the monic Hermite polynomials, the Christoffel-Darboux formula reads

$$\sum_{k=0}^{n-1} \frac{\pi_k(s) \pi_k(z)}{h_k} = \frac{\pi_n(s) \pi_{n-1}(z) - \pi_{n-1}(s) \pi_n(z)}{h_{n-1} (s - z)}$$

Multiply both sides by $e^{-s^2}$ and integrate over $\mathbb{R}$. On the left-hand side, only the $k = 0$ term survives because

$$\int_{-\infty}^{\infty} \pi_k(s) e^{-s^2} ds = 0$$

for $k \ge 1$, and since $\pi_0 = 1$ and $h_0 = \sqrt{\pi}$, the integral of the $k = 0$ term equals 1. On the right-hand side, using the fact that

$$\int_{-\infty}^{\infty} \frac{\pi_m(s) e^{-s^2}}{s - z} ds = -q_m(z)$$

we obtain

$$1 = \frac{-\pi_{n-1}(z) q_n(z) + \pi_n(z) q_{n-1}(z)}{h_{n-1}}$$

Hence

$$\pi_n(z) q_{n-1}(z) - \pi_{n-1}(z) q_n(z) = h_{n-1}$$

Step 3. Using $H_k = 2^k \pi_k$ and $Q_k = -e^{z^2} 2^k q_k$:

$$\Phi_n(z) = Q_n(z) H_{n-1}(z) - Q_{n-1}(z) H_n(z)$$

$$\Phi_n(z) = e^{z^2} 2^{2n-1} (\pi_n(z) q_{n-1}(z) - \pi_{n-1}(z) q_n(z))$$

By Step 2, this equals

$$e^{z^2} 2^{2n-1} h_{n-1} = e^{z^2} 2^{2n-1} \cdot 2^{-(n-1)} (n-1)! \sqrt{\pi} = e^{z^2} 2^n (n-1)! \sqrt{\pi}$$

Step 4. Therefore,

$$e^{-z^2} \Phi_n(z) \equiv 2^n (n-1)! \sqrt{\pi}$$

on $\mathbb{C} \setminus \mathbb{R}$, and in particular,

$$\lim_{|z| \to \infty} e^{-z^2} \Phi_n(z) = 2^n (n-1)! \sqrt{\pi}$$

Final Answer: True.