Let $\Theta_{\ell m}(x)$ denote the normalized associated Legendre functions on $x \in [-1,1]$ for integers $\ell \geq m \geq 0$:

$$\Theta_{\ell m}(x) = \sqrt{\frac{2\ell+1}{2} \cdot \frac{(\ell-m)!}{(\ell+m)!}} \cdot P_\ell^m(x)$$

where $P_\ell^m$ are the Ferrers associated Legendre functions. The normalized functions $\Theta_{\ell m}$ satisfy the three-term recurrence relation:

$$x \Theta_{\ell m}(x) = A_{\ell m} \Theta_{\ell+1,m}(x) + B_{\ell m} \Theta_{\ell-1,m}(x)$$

with coefficients $A_{\ell m}$ and $B_{\ell m}$ depending on $\ell$ and $m$.

For fixed $m \geq 1$, define $F_\ell^m$ for $\ell \geq m+2$ by:

$$F_\ell^m(x) = \Theta_{\ell m}(x) - \alpha_{\ell m} \Theta_{\ell-2,m}(x)$$

where $\alpha_{\ell m} = \frac{(\ell+m)(\ell-m)}{(2\ell-1)(2\ell+1)}$.

Claim: For all $\ell \geq m+3$ and all $m \geq 1$, there exists a two-term recurrence:

$$x F_\ell^m(x) = C_{\ell m} F_{\ell+1}^m(x) + D_{\ell m} F_{\ell-1}^m(x)$$

for appropriate constants $C_{\ell m}$ and $D_{\ell m}$ that depend only on $\ell$ and $m$.

Determine with rigorous proof whether the claim is True or False.

Answer: FALSE

Let $A_{\ell m},B_{\ell m}$ be the standard coefficients

$$A_{\ell m}=\sqrt{\frac{(\ell-m+1)(\ell+m+1)}{(2\ell+1)(2\ell+3)}},\qquad B_{\ell m}=\sqrt{\frac{(\ell-m)(\ell+m)}{(2\ell-1)(2\ell+1)}}.$$

With $\alpha_{\ell m}=\frac{(\ell+m)(\ell-m)}{(2\ell-1)(2\ell+1)}$, expand

$$xF_\ell^m=x\Theta_{\ell m}-\alpha_{\ell m}x\Theta_{\ell-2,m}$$

$$=A_{\ell m}\Theta_{\ell+1,m}+\bigl(B_{\ell m}-\alpha_{\ell m}A_{\ell-2,m}\bigr)\Theta_{\ell-1,m}-\alpha_{\ell m}B_{\ell-2,m}\Theta_{\ell-3,m}.$$

If there were constants $C_{\ell m},D_{\ell m}$ with

$$xF_\ell^m=C_{\ell m}F_{\ell+1}^m+D_{\ell m}F_{\ell-1}^m,$$

then expanding the right-hand side gives

$$C_{\ell m}\Theta_{\ell+1,m}+\bigl(-C_{\ell m}\alpha_{\ell+1,m}+D_{\ell m}\bigr)\Theta_{\ell-1,m}-D_{\ell m}\alpha_{\ell-1,m}\Theta_{\ell-3,m}.$$

Matching the $\Theta_{\ell+1,m}$ and $\Theta_{\ell-3,m}$ coefficients forces

$$C_{\ell m}=A_{\ell m},\qquad D_{\ell m}=\frac{\alpha_{\ell m}}{\alpha_{\ell-1,m}}\,B_{\ell-2,m}.$$

Matching the $\Theta_{\ell-1,m}$ coefficient also forces

$$D_{\ell m}=B_{\ell m}-\alpha_{\ell m}A_{\ell-2,m}+A_{\ell m}\alpha_{\ell+1,m}.$$

So a necessary condition for the claimed two-term recurrence is that these two formulas for $D_{\ell m}$ agree for all $\ell\ge m+3$.

  

They do not. Take $m=1,\ell=4$ (allowed since $\ell\ge m+3$). Then

$$D_{4,1}=\frac{\alpha_{4,1}}{\alpha_{3,1}}B_{2,1}=\frac{5\sqrt5}{24}\approx0.465847,$$

but the other forced value is

$$D_{4,1}=B_{4,1}-\alpha_{4,1}A_{2,1}+A_{4,1}\alpha_{5,1}=-\frac{2\sqrt{70}}{147}+\frac{16\sqrt{66}}{1089}+\frac{\sqrt{105}}{21}\approx0.493480.$$

These are not equal, so no such constants $C_{\ell m},D_{\ell m}$ can exist in general. Hence the claim is false.