For $n \ge 1$, define the Hermite function of the second kind as:

$$Q_n(z) = \int_{-\infty}^\infty \frac{e^{-t^2} H_n(t)}{z-t} dt.$$

Claim:

$$\lim_{z\to\infty} z^{n+1}Q_n(z) = \sqrt{\pi} n!.$$

Determine whether this claim is True or False, and give a rigorous proof of your conclusion.

Conclusion: True.

Fix $n\ge1$. For $z\in\mathbb C\setminus\mathbb R$, define the Hermite function of the second kind:

$$Q_n(z) = \int_{-\infty}^\infty \frac{e^{-t^2} H_n(t)}{z-t} dt$$

and set $\rho(z)=e^{-z^2}$.

In the Hermite case $(a,b)=(-\infty,\infty)$, so the domain condition $z\notin[a,b]$ means $z\in\mathbb C\setminus\mathbb R$. Taking $y_n(t)=H_n(t)$ and $\rho(t)=e^{-t^2}$, Nikiforov and Uvarov (Special Functions of Mathematical Physics, Birkhäuser, 1988, Chapter II, §11, Eq. 7) prove that:

$$Q_n^{NU}(z)\sim-\frac{d_n^2}{a_n\rho(z)z^{n+1}}\left(1+O(z^{-1})\right), \quad z\to\infty, \ z\in\mathbb C\setminus\mathbb R$$

where $a_n$ is the leading coefficient of $y_n$ and $d_n^2 = \int_{-\infty}^{\infty}\rho(t)y_n(t)^2dt$.

Since $1/(z-t)=-1/(t-z)$, the function $Q_n(z)$ satisfies the exact relation

$$Q_n(z)=-\int_{-\infty}^{\infty}\frac{\rho(t)y_n(t)}{t-z}dt=-\rho(z)Q_n^{NU}(z).$$

Multiplying the cited asymptotic by $-\rho(z)$ and using the exact identity $Q_n(z)=-\rho(z)Q_n^{NU}(z)$ rescales the asymptotic expansion by the factor $-\rho(z)$:

$$Q_n(z)\sim\frac{d_n^2}{a_n}z^{-(n+1)}\left(1+O(z^{-1})\right)$$

hence $\lim_{z\to\infty}z^{n+1}Q_n(z)=d_n^2/a_n$.

For Hermite polynomials, the leading coefficient is $a_n = 2^n$ and the square norm is $d_n^2 = \sqrt{\pi} 2^n n!$. Substituting these values yields:

$$\lim_{z\to\infty} z^{n+1} Q_n(z) = \frac{\sqrt{\pi} 2^n n!}{2^n} = \sqrt{\pi} n!$$

This matches the claim.