Let $L_n^{(\alpha)}(z)$ be the Laguerre polynomials. For $\text{Re}(\alpha) > -1$ and $z \in \mathbb{C} \setminus [0, \infty)$, the Laguerre function of the second kind is defined by:

$$Q_n^{(\alpha)}(z) = \int_0^\infty \frac{t^\alpha e^{-t} L_n^{(\alpha)}(t)}{z - t} dt$$


Define the function:

$$\phi_n(z) = z \frac{d}{dz} Q_n^{(\alpha)}(z) + (n+1) Q_{n+1}^{(\alpha)}(z) - (n + \alpha + 1 - z) Q_n^{(\alpha)}(z)$$

Claim: For all $n \ge 0$, the function $\phi_n(z)$ is identically zero on its domain.

Determine whether the claim is true or false, and give a rigorous proof.


Final Answer: False.

Proof. Let $w(t) = t^\alpha e^{-t}$ be the weight function.

Step 1. Differentiate under the integral.

For $z$ in any compact subset $K$ of $\mathbb{C} \setminus [0, \infty)$, the distance $d(K, [0, \infty)) = \delta > 0$ ensures $|z - t| \ge \delta$. This allows the interchange of the derivative and the integral by the dominated convergence theorem. Using the definition $Q_n^{(\alpha)}(z) = \int_0^\infty \frac{w(t) L_n^{(\alpha)}(t)}{z-t} dt$:

$$Q_n^{(\alpha)\prime}(z) = \frac{d}{dz} \int_0^\infty w(t) L_n^{(\alpha)}(t) (z-t)^{-1} dt = -\int_0^\infty \frac{w(t) L_n^{(\alpha)}(t)}{(z-t)^2} dt$$

Multiplying by $z$ and using the identity $z = (z-t) + t$:

$$z Q_n^{(\alpha)\prime}(z) = -\int_0^\infty \frac{(z-t) w(t) L_n^{(\alpha)}(t)}{(z-t)^2} dt - \int_0^\infty \frac{t w(t) L_n^{(\alpha)}(t)}{(z-t)^2} dt$$

$$z Q_n^{(\alpha)\prime}(z) = -Q_n^{(\alpha)}(z) - \int_0^\infty \frac{t w(t) L_n^{(\alpha)}(t)}{(z-t)^2} dt$$

Step 2. Integration by parts.

Let $I = \int_0^\infty \frac{t w(t) L_n^{(\alpha)}(t)}{(z-t)^2} dt$. Since $\frac{d}{dt} \left( \frac{1}{z-t} \right) = \frac{1}{(z-t)^2}$, integration by parts gives:

$$I = \left[ \frac{t^{\alpha+1} e^{-t} L_n^{(\alpha)}(t)}{z-t} \right]_0^\infty - \int_0^\infty \frac{(t^{\alpha+1} e^{-t} L_n^{(\alpha)}(t))'}{z-t} dt$$

For $\text{Re}(\alpha) > -1$, the boundary term vanishes. Applying the derivative identity $(t^{\alpha+1} e^{-t} L_n^{(\alpha)}(t))' = t^\alpha e^{-t} [ (n + \alpha + 1 - t) L_n^{(\alpha)}(t) - (n + \alpha) L_{n-1}^{(\alpha)}(t) ]$ and the standard three-term recurrence relation:

$$(n + \alpha + 1 - t) L_n^{(\alpha)}(t) - (n + \alpha) L_{n-1}^{(\alpha)}(t) = (n+1) L_{n+1}^{(\alpha)}(t) - n L_n^{(\alpha)}(t)$$

Thus, the integral $I$ becomes:

$$I = -\int_0^\infty \frac{w(t) [ (n+1) L_{n+1}^{(\alpha)}(t) - n L_n^{(\alpha)}(t) ]}{z-t} dt = -(n+1) Q_{n+1}^{(\alpha)}(z) + n Q_n^{(\alpha)}(z)$$

Step 3. Combine and evaluate $\phi_n(z)$.

Substituting $I$ back into the equation for $z Q_n^{(\alpha)\prime}(z)$:

$$z Q_n^{(\alpha)\prime}(z) = -Q_n^{(\alpha)}(z) - [ -(n+1) Q_{n+1}^{(\alpha)}(z) + n Q_n^{(\alpha)}(z) ]$$

$$z Q_n^{(\alpha)\prime}(z) = (n+1) Q_{n+1}^{(\alpha)}(z) - (n+1) Q_n^{(\alpha)}(z)$$

Now, substitute this into the definition of $\phi_n(z)$:

$$\phi_n(z) = [ (n+1) Q_{n+1}^{(\alpha)}(z) - (n+1) Q_n^{(\alpha)}(z) ] + (n+1) Q_{n+1}^{(\alpha)}(z) - (n + \alpha + 1 - z) Q_n^{(\alpha)}(z)$$

$$\phi_n(z) = 2(n+1) Q_{n+1}^{(\alpha)}(z) - (2n + \alpha + 2 - z) Q_n^{(\alpha)}(z)$$

Conclusion.

To show $\phi_n$ is not identically zero, consider $n=0$ as $z \to \infty$. Expanding the kernel as $\frac{1}{z-t} = \frac{1}{z} + \frac{t}{z^2} + O(z^{-3})$, we find $Q_1^{(\alpha)}(z) = O(z^{-2})$ due to the orthogonality of $L_1^{(\alpha)}(t)$ against constants. For $Q_0^{(\alpha)}(z)$, we have:

$$Q_0^{(\alpha)}(z) = \frac{1}{z}\int_0^\infty t^\alpha e^{-t} dt + O(z^{-2}) = \frac{\Gamma(\alpha+1)}{z} + O(z^{-2})$$

Substituting these into the formula for $\phi_0(z)$:

$$\phi_0(z) = 2Q_1^{(\alpha)}(z) + (z - \alpha - 2)Q_0^{(\alpha)}(z)$$

$$\phi_0(z) = O(z^{-2}) + (z - \alpha - 2) \left( \frac{\Gamma(\alpha+1)}{z} + O(z^{-2}) \right) = \Gamma(\alpha+1) + O(z^{-1})$$

As $z \to \infty$, $\phi_0(z) \to \Gamma(\alpha+1) \neq 0$. Thus, $\phi_0$ is not identically zero, proving the claim is false.