Let $\Theta_{\ell m}(x)$ denote the normalized associated Legendre functions on $x\in[-1,1]$ for integers $\ell\ge m\ge0$, defined by

$$\Theta_{\ell m}(x)=\sqrt{\frac{2\ell+1}{2}\frac{(\ell-m)!}{(\ell+m)!}}\,P_\ell^m(x),$$

where $P_\ell^m(x)$ are the standard associated Legendre functions. For fixed $m\ge0$ and any $x_0\in(-1,1)$, define the diagonal kernel value

$$K_N^{(m)}(x_0,x_0)=\sum_{\ell=m}^N\Theta_{\ell m}^2(x_0).$$

Claim

There exists a constant $C(x_0,m)>0$ such that

$$\liminf_{N\to\infty}\frac{K_N^{(m)}(x_0,x_0)}{N}\ge C(x_0,m).$$

Determine, with rigorous proof, whether this claim is True or False.

Conclusion True.

Let $\Theta_{\ell m}(x)=\sqrt{\frac{2\ell+1}{2}\frac{(\ell-m)!}{(\ell+m)!}}\,P_\ell^m(x)$ for integers $\ell\ge m\ge0$. Fix $m\ge0$ and $x_0\in(-1,1)$, and define
$$K_N^{(m)}(x_0,x_0)=\sum_{\ell=m}^N\Theta_{\ell m}(x_0)^2.$$

Since $x_0\in(-1,1)$, there is a unique $\theta_0\in(0,\pi)$ with $x_0=\cos\theta_0$. Using the Jacobi representation
$$P_\ell^m(x)=(-1)^m2^{-m}(1-x^2)^{m/2}\frac{(\ell+m)!}{\ell!}\,P_{\ell-m}^{(m,m)}(x),$$
we have
$$\Theta_{\ell m}(x_0)=A_{\ell,m}(x_0)\,P_{\ell-m}^{(m,m)}(x_0),$$
where
$$A_{\ell,m}(x_0)=(-1)^m2^{-m}(1-x_0^2)^{m/2}\sqrt{\frac{2\ell+1}{2}\frac{(\ell-m)!}{(\ell+m)!}}\frac{(\ell+m)!}{\ell!}.$$

By Stirling's formula with fixed $m$ (so all implied constants are uniform in $\ell$), there exists $a_m(x_0)>0$ such that
$$A_{\ell,m}(x_0)=a_m(x_0)\sqrt{\ell}\,(1+O(\ell^{-1})).$$

By SzegÅ‘ (Orthogonal Polynomials, Thm. 8.21.8, Eq. 8.21.10) specialized to $\alpha=\beta=m$ and $n=\ell-m$, there exist $b_m(\theta_0)>0$ (any sign absorbed into the phase) and $\psi_m(\theta_0)\in\mathbb{R}$ such that
$$P_{\ell-m}^{(m,m)}(\cos\theta_0)=(\ell-m)^{-1/2}b_m(\theta_0)\cos((\ell-m)\theta_0+\psi_m(\theta_0))+O(\ell^{-3/2}).$$
Rewriting $(\ell-m)\theta_0+\psi_m(\theta_0)=\ell\theta_0+\phi$ for $\phi=\psi_m(\theta_0)-m\theta_0$, this becomes
$$P_{\ell-m}^{(m,m)}(\cos\theta_0)=(\ell-m)^{-1/2}b_m(\theta_0)\cos(\ell\theta_0+\phi)+O(\ell^{-3/2}).$$

Since $\sqrt{\ell}(\ell-m)^{-1/2}=1+O(\ell^{-1})$, multiplying the two asymptotics gives
$$\Theta_{\ell m}(x_0)=M(x_0,m)\cos(\ell\theta_0+\phi)+O(\ell^{-1})$$
where we take $M(x_0,m)=a_m(x_0)b_m(\theta_0)>0$.

Squaring yields
$$\Theta_{\ell m}(x_0)^2=M(x_0,m)^2\cos^2(\ell\theta_0+\phi)+O(\ell^{-1}),$$
and summing from $\ell=m$ to $N$ gives
$$K_N^{(m)}(x_0,x_0)=M(x_0,m)^2\sum_{\ell=m}^N\cos^2(\ell\theta_0+\phi)+O(\log N).$$

Since $\cos^2 t=\frac{1}{2}+\frac{1}{2}\cos(2t)$, we have
$$\frac{1}{N}\sum_{\ell=m}^N\cos^2(\ell\theta_0+\phi)=\frac{1}{2}+\frac{1}{2N}\sum_{\ell=m}^N\cos(2\ell\theta_0+2\phi).$$
For $\theta_0\in(0,\pi)$, $e^{i2\theta_0}\neq1$, so the geometric sum $\sum_{\ell=m}^N e^{i2\ell\theta_0}=e^{i2m\theta_0}\frac{1-e^{i2(N-m+1)\theta_0}}{1-e^{i2\theta_0}}$ is uniformly bounded in $N$. Thus $\frac{1}{N}\sum_{\ell=m}^N\cos(2\ell\theta_0+2\phi)\to0$, and
$$\frac{1}{N}\sum_{\ell=m}^N\cos^2(\ell\theta_0+\phi)\to\frac{1}{2}.$$

Therefore,
$$\lim_{N\to\infty}\frac{K_N^{(m)}(x_0,x_0)}{N}=\frac{1}{2}\,M(x_0,m)^2>0,$$
proving the claim with $C(x_0,m)=\frac{1}{2}\,M(x_0,m)^2$.