Let $P_n^{(\alpha,\beta)}(x)$ be the Jacobi polynomials orthogonal on $[-1,1]$ with respect to $p(x) = (1-x)^\alpha(1+x)^\beta$. 

Define a new weight function by multiplying the original weight by a linear factor that does not change sign on the interval:

$$\hat{p}(x) = (x+2)p(x)$$

Consider the following claim:

The polynomials $\hat{P}_n(x)$ orthogonal with respect to $\hat{p}(x)$ can be expressed as a linear combination of only two consecutive original Jacobi polynomials in the form:

$$\hat{P}_n(x) = P_n^{(\alpha,\beta)}(x) + \kappa_n P_{n-1}^{(\alpha,\beta)}(x)$$

for some constant $\kappa_n$.

Determine, with rigorous proof, whether the claim is **True or False**.

The claim is **False**

Step 1. Work in the Jacobi inner product $(f,g) = \int_{-1}^1 f(x)g(x)p(x) dx$ with $p(x) = (1-x)^\alpha(1+x)^\beta$, where $\alpha, \beta > -1$. Let $P_n(x) = P_n^{(\alpha,\beta)}(x)$ and $h_n = (P_n, P_n) > 0$.

Step 2. The modified weight is $\hat{p}(x) = (x+2)p(x)$. Orthogonality for $\hat{P}_n$ requires:

$\int_{-1}^1 \hat{P}_n(x) P_k(x) (x+2) p(x) dx = 0$ for all $k = 0, 1, \dots, n-1$.

Assume the claim: $\hat{P}_n = P_n + \kappa_n P_{n-1}$.

Step 3. Use the three-term recurrence for Jacobi polynomials:

$xP_k = A_k P_{k+1} + B_k P_k + C_k P_{k-1}$ for $k \ge 0$, where $C_0 = 0$.

The coefficient $A_k = \frac{2(k+1)(k+\alpha+\beta+1)}{(2k+\alpha+\beta+1)(2k+\alpha+\beta+2)}$ is non-zero for all $k \ge 0$.

Step 4. Check orthogonality for $k = n-2$ assuming $n \ge 2$.

Compute:

$\int_{-1}^1 (P_n + \kappa_n P_{n-1}) P_{n-2} (x+2) p(x) dx = (P_n + \kappa_n P_{n-1}, xP_{n-2}) + 2(P_n + \kappa_n P_{n-1}, P_{n-2})$.

The second term is $0$ by standard orthogonality. Using the recurrence for $xP_{n-2}$:

$(P_n + \kappa_n P_{n-1}, A_{n-2}P_{n-1} + B_{n-2}P_{n-2} + C_{n-2}P_{n-3}) = \kappa_n A_{n-2} (P_{n-1}, P_{n-1}) = \kappa_n A_{n-2} h_{n-1}$.

For this to equal $0$, since $A_{n-2} \ne 0$ and $h_{n-1} > 0$, we must have $\kappa_n = 0$.

Step 5. Check orthogonality for $k = n-1$ with $\kappa_n = 0$.

The condition becomes:

$\int_{-1}^1 P_n(x) P_{n-1}(x) (x+2) p(x) dx = (P_n, xP_{n-1}) + 2(P_n, P_{n-1}) = (P_n, xP_{n-1})$.

Using the recurrence for $xP_{n-1}$:

$(P_n, A_{n-1}P_n + B_{n-1}P_{n-1} + C_{n-1}P_{n-2}) = A_{n-1} (P_n, P_n) = A_{n-1} h_n$.

Since $A_{n-1} \ne 0$ and $h_n > 0$, the result is non-zero, creating a contradiction.

Step 6. Final Conclusion: False.