Let $L_n^{(\alpha)}(t)$ be the Laguerre polynomials. For $\mathrm{Re}(\alpha) > -1$ and $z \in \mathbb{C} \setminus [0, \infty)$, define the Laguerre function of the second kind:

$$Q_n^{(\alpha)}(z) = \int_0^\infty \frac{t^\alpha e^{-t} L_n^{(\alpha)}(t)}{z - t} dt$$

Using the principal branch for $t^\alpha$, set $\rho(z) = z^\alpha e^{-z}$, $\sigma(z) = z$, $\tau(z) = \alpha + 1 - z$, and define the differential operator:

$$\mathcal{D}[f](z) = \sigma(z) f'(z) + (\sigma'(z) - \tau(z)) f(z)$$

Let $w_n(z) = \rho(z) Q_n^{(\alpha)}(z)$. Determine whether the following claim is true or false, and provide a rigorous proof:

$$\mathcal{D}[w_n](z) = \Gamma(\alpha + 1) \delta_{n0} - n w_n(z) \quad (n \ge 0)$$

where $\delta_{n0}$ is the Kronecker delta.

Conclusion: false.

Fix Re($\alpha$) > -1 and $z \in \mathbb C \setminus [0, \infty)$. Let $\rho(z) = z^\alpha e^{-z}$ and $w_n(z) = \rho(z) Q_n^{(\alpha)}(z)$. Define $\mathcal D f(z) = z f'(z) + (z - \alpha) f(z)$.

Step 1. Reduction to a first-order ODE.

With $w_n = \rho Q_n$ and $\rho'(z) = \rho(z)(\alpha/z - 1)$, a direct calculation yields

$\mathcal D w_n = z(\rho Q_n)'(z) + (z - \alpha) \rho(z) Q_n(z) = \rho(z) z Q_n^{(\alpha)'}(z)$.

The identity $\mathcal D[w_n] = \Gamma(\alpha + 1) \delta_{n0} - n w_n$ is therefore equivalent to

$z Q_n^{(\alpha)'}(z) + n Q_n^{(\alpha)}(z) = \Gamma(\alpha + 1) \delta_{n0} \rho(z)^{-1}$.

For $n \ge 1$ this reduces to the homogeneous ODE $z Q_n^{(\alpha)'}(z) + n Q_n^{(\alpha)}(z) = 0$, which implies

$Q_n^{(\alpha)}(z) = c_n z^{-n}$.

Step 2. Asymptotics 

Nikiforov–Uvarov, 1988, Chapter II, §11, Eq.(7), define the function of the second kind as

$Q_n^{NU}(z) = \frac{1}{\rho(z)} \int_a^b \frac{\rho(t) y_n(t)}{z - t} dt$

and prove the asymptotic (Eq.(7))

$Q_n^{NU}(z) \sim -\frac{d_n^2}{a_n \rho(z) z^{n+1}} (1 + O(z^{-1}))$ as $z \to \infty$ with $z \notin [a, b]$.

In the Laguerre case where $(a, b) = (0, \infty)$, $y_n(t) = L_n^{(\alpha)}(t)$ and $\rho(t) = t^\alpha e^{-t}$. Our function $Q_n^{(\alpha)}(z)$ is the numerator integral

$Q_n^{(\alpha)}(z) = \int_0^\infty \frac{\rho(t) L_n^{(\alpha)}(t)}{z - t} dt = \rho(z) Q_n^{NU}(z)$.

Multiplying the NU asymptotic by $\rho(z)$ gives

$Q_n^{(\alpha)}(z) \sim -\frac{d_n^2}{a_n z^{n+1}} (1 + O(z^{-1}))$.

Given $a_n = (-1)^n / n!$ and $d_n^2 = \Gamma(n + \alpha + 1) / n!$, the leading coefficient is

$C_n = - \frac{d_n^2}{a_n} = (-1)^{n+1} \Gamma(n + \alpha + 1) \neq 0$.

Thus, $Q_n^{(\alpha)}(z) \sim C_n z^{-(n+1)}$.

Step 3. Conclusion.

Step 1 forces $Q_n^{(\alpha)}(z) = c_n z^{-n}$ for $n \ge 1$. However, Step 2 shows that the actual leading order behavior is $z^{-(n+1)}$ with a non-zero coefficient $C_n$. These power laws are incompatible for all $n \ge 1$. This contradiction proves that the claimed identity is false.