Let

$$I_n = n^2 \int_{0}^{1}\frac{x^{n}}{1+2x+\frac{2}{n}}\,dx.$$

Compute

$$L = \lim_{n\to\infty}\Big( I_n - \frac{n}{3}\Big).$$

Substitute $x = e^{-t/n}$. Then $x^n = e^{-t}$, $dx = -(1/n) e^{-t/n} dt$, and the limits $x: 0 \to 1$ become $t: \infty \to 0$, so

$$I_n = n \int_0^\infty e^{-t} \cdot \frac{e^{-t/n}}{1 + 2 e^{-t/n} + 2/n} dt$$

Expand the rational part of the integrand for large $n$:

$$e^{-t/n} = 1 - \frac{t}{n} + O\left(\frac{t^2}{n^2}\right)$$

The numerator is $1 - \frac{t}{n} + O(\frac{t^2}{n^2})$, and the denominator is

$$1 + 2\left(1 - \frac{t}{n} + O\left(\frac{t^2}{n^2}\right)\right) + \frac{2}{n} = 3 + \frac{2 - 2t}{n} + O\left(\frac{t^2}{n^2}\right)$$

Thus, the fraction expands as:

$$\frac{e^{-t/n}}{1 + 2 e^{-t/n} + 2/n} = \frac{1 - \frac{t}{n}}{3(1 + \frac{2-2t}{3n})} + O\left(\frac{t^2}{n^2}\right) = \frac{1}{3} - \frac{t+2}{9n} + O\left(\frac{1+t^2}{n^2}\right)$$

The remainder term $R(n, t) = O((1+t^2)/n^2)$ is uniformly bounded in $t$ after multiplying by the factor $e^{-t}$, ensuring the integral of the remainder is $O(n^{-2})$.

Integrate against $e^{-t}$:

$$\int_0^\infty e^{-t} \left( \frac{1}{3} - \frac{t + 2}{9n} \right) dt + O(n^{-2}) = \frac{1}{3} \int_0^\infty e^{-t} dt - \frac{1}{9n} \int_0^\infty e^{-t} (t + 2) dt + O(n^{-2})$$

Using the standard moments $\int_0^\infty e^{-t} dt = 1$ and $\int_0^\infty t e^{-t} dt = 1$:

$$\int_0^\infty e^{-t} (t + 2) dt = 1 + 2 = 3$$

The integral evaluates to:

$$\frac{1}{3} - \frac{3}{9n} + O(n^{-2}) = \frac{1}{3} - \frac{1}{3n} + O(n^{-2})$$

Multiply by the leading factor $n$:

$$I_n = \frac{n}{3} - \frac{1}{3} + O(n^{-1})$$

Hence,

$$L = \lim_{n \to \infty} \left( I_n - \frac{n}{3} \right) = -\frac{1}{3}$$