Let
\[
I_n \;=\; n^2 \int_{0}^{1}\frac{x^{n}}{1+2x+\frac{2}{n}}\,dx.
\]
Compute
\[
L \;=\; \lim_{n\to\infty}\Big( I_n - \tfrac{n}{3}\Big).
\]

\begin{enumerate}
    \item Split the integrand at the value of the denominator at $x=1$:
    \[
    \frac{1}{1+2x+\tfrac{2}{n}}
    \;=\; \frac{1}{3+\tfrac{2}{n}}
    \;+\;\Bigg(\frac{1}{1+2x+\tfrac{2}{n}}-\frac{1}{3+\tfrac{2}{n}}\Bigg).
    \]

    \item Evaluate the ``constant'' piece exactly:
    \[
    n^2\!\int_0^1 \frac{x^n}{3+\tfrac{2}{n}}\,dx
    \;=\; \frac{n^2}{3+\tfrac{2}{n}}\cdot\frac{1}{n+1}
    \;=\; \frac{n}{3}-\frac{2}{9}+O\!\Big(\frac{1}{n}\Big).
    \]

    \item Linearize the remainder around $x=1$:
    \[
    \frac{1}{1+2x+\tfrac{2}{n}}-\frac{1}{3+\tfrac{2}{n}}
    \;=\; -\,\frac{(1+2x+\tfrac{2}{n})-(3+\tfrac{2}{n})}{(1+2x+\tfrac{2}{n})(3+\tfrac{2}{n})}
    \;=\; -\,\frac{2(x-1)}{(3+\tfrac{2}{n})^2} \;+\; O\big((x-1)^2\big).
    \]

    \item Use the identity $(x-1)x^n = x^{n+1}-x^n$ to get an exact moment:
    \[
    n^2\!\int_0^1 x^n(x-1)\,dx
    \;=\; n^2\!\left(\frac{1}{n+2}-\frac{1}{n+1}\right)
    \;=\; \frac{n^2}{(n+1)(n+2)} \;=\; 1+O\!\Big(\frac{1}{n}\Big).
    \]

    \item Assemble the remainder contribution:
    \[
    n^2\!\int_0^1 x^n\!\left(\frac{1}{1+2x+\tfrac{2}{n}}-\frac{1}{3+\tfrac{2}{n}}\right)\!dx
    \;=\; -\,\frac{2}{(3+\tfrac{2}{n})^2}\cdot\Big[1+O\!\Big(\frac{1}{n}\Big)\Big]
    \;=\; -\frac{2}{9}+O\!\Big(\frac{1}{n}\Big).
    \]

    \item Add the two pieces:
    \[
    I_n \;=\; \Big(\frac{n}{3}-\frac{2}{9}\Big) \;+\; \Big(-\frac{2}{9}\Big) \;+\; O\!\Big(\frac{1}{n}\Big)
    \;=\; \frac{n}{3}-\frac{1}{3}+O\!\Big(\frac{1}{n}\Big).
    \]

    \item Take the limit:
    \[
    L \;=\; \lim_{n\to\infty}\Big(I_n-\tfrac{n}{3}\Big) \;=\; -\frac{1}{3}.
    \]
\end{enumerate}