Let $\phi(x) = e^{-x^2}$ be the weight function for the Hermite polynomials $H_n(x)$ on $(-\infty, \infty)$. For $z \in \mathbb{C} \setminus \mathbb{R}$, define the function

$$Q_n(z) = \int_{-\infty}^{\infty} \frac{e^{-t^2} H_n(t)}{z - t} dt.$$

Claim. For every $n \ge 1$, the function $Q_n(z)$ satisfies the asymptotic property

$$\lim_{z \to \infty} \frac{z Q_n(z)}{Q_{n-1}(z)} = n.$$

Determine, with rigorous justification, whether the claim is true or false.

The claim is True.

To determine the behavior of $Q_n(z)$ as $z \to \infty$, we utilize the geometric series expansion of the integrand's kernel. For sufficiently large $|z|$, the term $(z - t)^{-1}$ can be expressed as:

$$\frac{1}{z - t} = \frac{1}{z} \sum_{k=0}^{\infty} \left( \frac{t}{z} \right)^k = \sum_{k=0}^{\infty} \frac{t^k}{z^{k+1}}$$


For any integer $N \ge 0$, one has the exact identity:

$$\frac{1}{z-t}=\sum_{k=0}^{N}\frac{t^{k}}{z^{k+1}}+\frac{t^{N+1}}{z^{N+1}}\frac{1}{z-t}.$$

Taking $N=n$ and substituting into the definition of $Q_n(z)$ gives:

$$Q_n(z)=\sum_{k=0}^{n}\frac{1}{z^{k+1}}\int_{-\infty}^{\infty}e^{-t^2}H_n(t)t^{k}\,dt +\frac{1}{z^{n+1}}\int_{-\infty}^{\infty}\frac{e^{-t^2}H_n(t)t^{n+1}}{z-t}\,dt.$$

Since the sum is finite, the integrals may be taken term by term, and the last term is a remainder of order $O(z^{-n-2})$ as $z \to \infty$ with $z \in \mathbb{C} \setminus \mathbb{R}$.

By the structural property of orthogonality, the integral $\int_{-\infty}^{\infty} e^{-t^2} H_n(t) t^k dt$ vanishes for all $k < n$. The first non-vanishing term in the series occurs precisely when $k = n$. Therefore, the leading-order asymptotic behavior of $Q_n(z)$ is:

$$Q_n(z) \sim \frac{1}{z^{n+1}} \int_{-\infty}^{\infty} e^{-t^2} H_n(t) t^n dt$$

For the physicists' Hermite polynomials, the value of this integral is $\sqrt{\pi} n!$. Thus, the leading term is:

$$Q_n(z) \sim \frac{\sqrt{\pi} n!}{z^{n+1}}$$

Applying this result to the ratio in the claim:

$$\lim_{z \to \infty} \frac{z Q_n(z)}{Q_{n-1}(z)} = \lim_{z \to \infty} \frac{z \cdot \frac{\sqrt{\pi} n!}{z^{n+1}}}{\frac{\sqrt{\pi} (n-1)!}{z^n}} = \frac{n!}{(n-1)!} = n$$

Conclusion: True.